recursors_api/Recursors/recursor_rec_call.v
@@ -51,13 +51,13 @@ Fixpoint make_rec_call_aux (id_arg : ident) (rev_ids_local : list ident) (ty : t
   match hd with
   (* 1. If it is an iterated product or LetIn => accumulates arg  *)
   | tProd an A B =>
-      let* id_local s <- add_old_var (Some "local_arg") (mkdecl an None A) s in
+      let* id_local s := add_old_var (Some "local_arg") (mkdecl an None A) s in
       match make_rec_call_aux id_arg (id_local :: rev_ids_local) B s with
       | Some (ty, tm) => Some (tProd an A ty, tLambda an A tm)
       | None => None
       end
   | tLetIn an db A B =>
-      let* _ s <- add_old_var (Some "local_let") (mkdecl an (Some db) A) s in
+      let* _ s := add_old_var (Some "local_let") (mkdecl an (Some db) A) s in
       match make_rec_call_aux id_arg rev_ids_local B s with
       | Some (ty, tm) => Some (tLetIn an db A ty, tLetIn an db A tm)
       | None => None
@@ -88,7 +88,7 @@ Fixpoint make_rec_call_aux (id_arg : ident) (rev_ids_local : list ident) (ty : t
         (* 2.2.2 Check for further rec call recursively *)
         let compute_nested_rc (x : term) (e : state) : (option (term * term)) :=
           let anx := mkBindAnn nAnon Relevant in
-          let* id_farg s <- add_fresh_var (Some "rec_arg") (mkdecl anx None x) s in
+          let* id_farg s := add_fresh_var (Some "rec_arg") (mkdecl anx None x) s in
           match make_rec_call_aux id_farg [] (lift0 1 x) s with
           | Some (ty, tm) => Some (tLambda anx x ty, tLambda anx x tm)
           | None => None
